proved preservation of termination

Conversion/ATerm_of_String.v
@@ -12,6 +12,7 @@ Set Implicit Arguments.
 Require Import LogicUtil.
 Require Import RelUtil.
 Require Import SN.
+Require Import ListUtil.
 
 Section S.
 
@@ -20,30 +21,50 @@ Section S.
 
 Require Import Srs.
 
-Variable SSig : Signature.
+Variable SSig : VSignature.Signature.
 
-Notation string := (list SSig).
-Notation letter := (symbol SSig).
+Notation letter := (symbol SSig). Notation string := (list SSig).
 Notation srule := (rule SSig).
 
 (***********************************************************************)
 (** corresponding algebraic signature *)
 
-Require Import ATrs.
-
 Definition ar (s : letter) := 1.
+
+Require Import ATrs.
 
 Definition ASig_of_SSig := mkSignature ar (@VSignature.beq_symb_ok SSig).
 
 Notation ASig := ASig_of_SSig.
 
 Notation term := (term ASig). Notation terms := (vector term).
+Notation context := (context ASig).
 
+Require Import AUnary.
+
+Lemma is_unary_sig : is_unary ASig.
+
+Proof.
+intro. refl.
+Qed.
+
+Ltac arity := arity1 is_unary_sig.
+Ltac is_unary := try (exact is_unary_sig).
+
+Notation cont := (cont is_unary_sig).
+Notation term_ind_forall := (term_ind_forall is_unary_sig).
+ 
 Fixpoint term_of_string (s : string) : term :=
   match s with
     | nil => Var 0
     | a :: w => @Fun ASig a (Vcons (term_of_string w) Vnil)
   end.
+
+Lemma var_term_of_string : forall s, var (term_of_string s) = 0.
+
+Proof.
+induction s; auto.
+Qed.
 
 (*FIXME: does not work:
 Fixpoint string_of_term (t : term) : string :=
@@ -69,25 +90,46 @@ Proof.
 induction s; simpl; intros. refl. rewrite IHs. refl.
 Qed.
 
-Require Import VecUtil.
-Require Import Max.
-
-Ltac arity_1 := let f := fresh "f" in let v := fresh "v" in
-  intros f v; unfold arity in v; simpl in v; unfold ar in v; VSntac v;
-    let a := fresh "a" in let w := fresh "w" in
-      set (a := Vhead v); set (w := Vtail v); VOtac.
+Require Import NatUtil.
 
 Lemma term_of_string_epi : forall t, maxvar t = 0 ->
   term_of_string (string_of_term t) = t.
 
 Proof.
 intro t; pattern t; apply term_ind_forall; clear t.
-(* Var *)
 simpl in *. intros. subst. refl.
-(* Fun *)
-arity_1. rewrite H0. simpl. intros. apply args_eq. destruct H1.
-assert (maxvar a <= 0). rewrite <- H2. apply le_max_l.
-assert (h : maxvar a = 0). omega. rewrite H1. refl. hyp.
+intros f t IH. simpl. rewrite max_0_r. intro h. rewrite (IH h). refl.
+Qed.
+
+Implicit Arguments term_of_string_epi [t].
+
+Fixpoint string_of_cont (c : context) : string :=
+  match c with
+    | Hole => nil
+    | Cont f _ _ _ _ d _ => f :: string_of_cont d
+  end.
+
+Lemma string_of_term_cont : forall t,
+  string_of_term t = string_of_cont (cont t).
+
+Proof.
+apply term_ind_forall. refl. intros f t IH. simpl. rewrite IH. refl.
+Qed.
+
+Lemma string_of_term_fill : forall t c,
+  string_of_term (fill c t) = string_of_cont c ++ string_of_term t.
+
+Proof.
+induction c. refl. simpl. rewrite Vmap_first_cast. arity. simpl. rewrite IHc.
+refl.
+Qed.
+
+Lemma string_of_term_sub : forall s l,
+  string_of_term (sub s l) = string_of_term l ++ string_of_term (s (var l)).
+
+Proof.
+intro s. apply term_ind_forall. refl. intros f t IH. rewrite sub_fun. simpl.
+rewrite IH. refl.
 Qed.
 
 (***********************************************************************)
@@ -96,10 +138,10 @@ Qed.
 Definition cont_of_letter a :=
   @Cont ASig a 0 0 (refl_equal 1) (@Vnil term) Hole Vnil.
 
-Fixpoint cont_of_string (s : string) : context ASig :=
+Fixpoint cont_of_string (s : string) : context :=
   match s with
     | nil => Hole
-    | a :: w => AContext.comp (cont_of_letter a) (cont_of_string w)
+    | a :: w => comp (cont_of_letter a) (cont_of_string w)
   end.
 
 (***********************************************************************)
@@ -115,8 +157,7 @@ Definition subs_of_string s x :=
   end.
 
 Lemma term_sfill : forall sc s,
-  term_of_string (SContext.fill sc s) =
-  fill (cont_of_string (lft sc))
+  term_of_string (SContext.fill sc s) = fill (cont_of_string (lft sc))
   (sub (subs_of_string (rgt sc)) (term_of_string s)).
 
 Proof.
@@ -128,57 +169,132 @@ Qed.
 (***********************************************************************)
 (** rewriting *)
 
+Definition trs_of_srs R := map rule_of_srule R.
+
+Lemma rules_preserv_vars_trs_of_srs :
+  forall R, rules_preserv_vars (trs_of_srs R).
+
+Proof.
+unfold rules_preserv_vars. induction R; simpl; intuition.
+unfold rule_of_srule in H0. destruct a. simpl in H0. inversion H0.
+repeat rewrite vars_var; is_unary. repeat rewrite var_term_of_string.
+unfold incl; simpl; intuition.
+Qed.
+
+Ltac preserv_vars := try (apply rules_preserv_vars_trs_of_srs).
+
 Section red_of_sred.
 
-Variable S : list srule.
-
-Definition trs_of_srs := List.map rule_of_srule S.
-
-Notation R := trs_of_srs.
+Variable R : list srule.
 
 Lemma red_of_sred : forall x y,
-  Srs.red S x y -> red R (term_of_string x) (term_of_string y).
+  Srs.red R x y -> red (trs_of_srs R) (term_of_string x) (term_of_string y).
 
 Proof.
 intros. do 3 destruct H. decomp H. subst x. subst y. repeat rewrite term_sfill.
-apply red_rule. change (In (rule_of_srule (Srs.mkRule x0 x1)) R).
+apply red_rule. change (In (rule_of_srule (Srs.mkRule x0 x1)) (trs_of_srs R)).
 unfold trs_of_srs. apply in_map. exact H0.
 Qed.
 
-Lemma red_of_sred_rtc : forall x y,
-  Srs.red S # x y -> red R # (term_of_string x) (term_of_string y).
+Lemma rtc_red_of_sred : forall x y,
+  Srs.red R # x y -> red (trs_of_srs R) # (term_of_string x) (term_of_string y).
 
 Proof.
 intros. elim H; intros. apply rt_step. apply red_of_sred. exact H0.
 apply rt_refl. eapply rt_trans. apply H1. exact H3.
 Qed.
 
+Lemma sred_of_red0 : forall t u,
+  red0 (trs_of_srs R) t u -> Srs.red R (string_of_term t) (string_of_term u).
+
+Proof.
+intros. destruct H. redtac. subst. repeat rewrite string_of_term_fill.
+repeat rewrite string_of_term_sub. rewrite (rules_preserv_vars_var
+  is_unary_sig (rules_preserv_vars_trs_of_srs R) lr).
+set (c' := mkContext (string_of_cont c) (string_of_term (s (var l)))).
+change (Srs.red R (SContext.fill c' (string_of_term l))
+  (SContext.fill c' (string_of_term r))). apply Srs.red_rule. clear c'.
+destruct (in_map_elim lr). destruct H. destruct x. unfold rule_of_srule in H1.
+simpl in H1. inversion H1. repeat rewrite string_of_term_epi. hyp.
+Qed.
+
+Lemma rtc_sred_of_red0 : forall t u, red (trs_of_srs R) # t u ->
+  maxvar t = 0 -> Srs.red R # (string_of_term t) (string_of_term u).
+
+Proof.
+induction 1; intro. apply rt_step. apply sred_of_red0. unfold red0. intuition.
+apply rt_refl. apply rt_trans with (string_of_term y). auto.
+apply IHclos_refl_trans2. eapply rtc_red_maxvar0.
+apply rules_preserv_vars_trs_of_srs. apply H1. apply H.
+Qed.
+ 
 End red_of_sred.
 
 (***********************************************************************)
 (** reflexion of termination *)
 
-Variable D S : list srule.
+Variables E R : list srule.
 
-Notation E := (trs_of_srs D). Notation R := (trs_of_srs S).
-
-Lemma red_mod_of_sred_mod : forall x y,
-  Srs.red_mod D S x y -> red_mod E R (term_of_string x) (term_of_string y).
+Lemma red_mod_of_sred_mod : forall x y, Srs.red_mod E R x y ->
+  red_mod (trs_of_srs E) (trs_of_srs R) (term_of_string x) (term_of_string y).
 
 Proof.
 intros. do 2 destruct H. exists (term_of_string x0). split.
-apply red_of_sred_rtc. exact H. apply red_of_sred. exact H0.
+apply rtc_red_of_sred. exact H. apply red_of_sred. exact H0.
 Qed.
 
-Lemma WF_red_mod_of_WF_sred_mod : WF (red_mod E R) -> WF (Srs.red_mod D S).
+Lemma WF_red_mod_of_WF_sred_mod :
+  WF (red_mod (trs_of_srs E) (trs_of_srs R)) -> WF (Srs.red_mod E R).
 
 Proof.
 unfold WF. intro H.
-cut (forall t s, t = term_of_string s -> SN (Srs.red_mod D S) s).
+cut (forall t s, t = term_of_string s -> SN (Srs.red_mod E R) s).
 intros. apply H0 with (term_of_string x). refl.
 intro t. generalize (H t). induction 1. intros. apply SN_intro. intros.
 apply H1 with (term_of_string y). 2: refl. subst x. apply red_mod_of_sred_mod.
 exact H3.
+Qed.
+
+(***********************************************************************)
+(** preservation of termination *)
+
+Lemma sred_mod_of_red_mod0 : forall t u,
+  red_mod0 (trs_of_srs E) (trs_of_srs R) t u ->
+  Srs.red_mod E R (string_of_term t) (string_of_term u).
+
+Proof.
+intros. do 3 destruct H. exists (string_of_term x); split.
+apply rtc_sred_of_red0; hyp. apply sred_of_red0. unfold red0. intuition.
+eapply rtc_red_maxvar0. apply rules_preserv_vars_trs_of_srs. apply H0. apply H.
+Qed.
+
+Lemma WF_sred_mod_of_WF_red_mod :
+  WF (Srs.red_mod E R) -> WF (red_mod (trs_of_srs E) (trs_of_srs R)).
+
+Proof.
+intro. rewrite WF_red_mod0; is_unary; preserv_vars.
+cut (forall s, SN (Srs.red_mod E R) s -> forall t, maxvar t = 0 ->
+  t = term_of_string s -> SN (red_mod0 (trs_of_srs E) (trs_of_srs R)) t).
+(* cut correctness *)
+intros. intro t. destruct (eq_nat_dec (maxvar t) 0). Focus 2.
+apply SN_intro. intros. destruct H1. absurd_arith.
+apply H0 with (string_of_term t). apply H. hyp. rewrite term_of_string_epi.
+refl. hyp.
+(* proof with cut *)
+induction 1; intros. apply SN_intro; intros. assert (h : maxvar y = 0).
+apply (red_mod0_maxvar (rules_preserv_vars_trs_of_srs E)
+  (rules_preserv_vars_trs_of_srs R) H4). rewrite <- (term_of_string_epi h).
+apply H1 with (string_of_term y). 3: refl.
+2: rewrite (term_of_string_epi h); hyp. rewrite <- (string_of_term_epi x).
+apply sred_mod_of_red_mod0. subst. hyp.
+Qed.
+
+Lemma WF_conv :
+  WF (Srs.red_mod E R) <-> WF (red_mod (trs_of_srs E) (trs_of_srs R)).
+
+Proof.
+split; intro. apply WF_sred_mod_of_WF_red_mod. hyp.
+apply WF_red_mod_of_WF_sred_mod. hyp.
 Qed.
 
 End S.
